ulib/FStar.Reflection.Types.fsti
@@ -31,6 +31,7 @@ assume new type sigelt // called `def` in the paper, but we keep the internal na
 assume new type ctx_uvar_and_subst
 assume new type letbinding
 
+assume new type __ident
 assume new type universe_uvar
 assume new type universe
 
