ulib/FStar.Syntax.Syntax.fsti
@@ -7,5 +7,5 @@ type subst_elt =
   | NM : namedv -> int -> subst_elt
   | NT : namedv -> term -> subst_elt
   | UN : int -> universe -> subst_elt
-  | UD : univ_name -> int -> subst_elt
+  | UD : __ident -> int -> subst_elt
 type subst_t = list subst_elt
